theories/CTree/Logic/Iter.v
@@ -1,399 +1,264 @@
-Section CtlAuIter.
+From Coinduction Require Import
+  coinduction lattice.
+
+From CTree Require Import
+  Events.Core
+  CTree.Core
+  CTree.Equ
+  CTree.SBisim
+  CTree.Logic.Trans
+  CTree.Logic.CanStep
+  CTree.Logic.AX
+  CTree.Logic.AF
+  CTree.Logic.AG
+  CTree.Logic.EX
+  CTree.Logic.EF
+  CTree.Logic.Bind
+  Logic.Ctl.
+
+Generalizable All Variables.
+
+Import CTreeNotations CtlNotations.
+Local Open Scope ctl_scope.
+Local Open Scope ctree_scope.
+
+Section IterLemmas.
   Context {E: Type} {HE: Encode E}.
 
-  Lemma au_iter_now{X I} Ri (Rv: relation (I * World E)) (i: I) w (k: I -> ctree E (I + X)) (φ: ctlf E (I + X)):
+  (* AX *)
+  Lemma axl_iter{X I} Ri (Rv: relation (I * World E)) (i: I) w (k: I -> ctree E (I + X)) (φ ψ: ctll E):
     well_founded Rv ->
     Ri i w ->    
     (forall (i: I) w,
         Ri i w ->
-        <( {k i}, w |= AF φ \/ 
-                    AF AX done
-                      {fun (x: I + X) (w': World E) => True})>) ->
-
-    <( {iter k i}, w |= AF φ )>.
-                                                
-  (* Termination lemma for [iter] *)
-  (* [Ri: I -> World E -> Prop] loop invariant (left).
-     [Rr: X -> World E -> Prop] loop postcondition (right).
-     [Rv: (I * World E) -> (I * World E) -> Prop)] loop variant (left). *)
-  Lemma au_iter_done{X I} Ri Rr (Rv: relation (I * World E)) (i: I) w (k: I -> ctree E (I + X)) φ:
-    (forall (i: I) w,
-        Ri i w ->
-        <( {k i}, w |= base φ AU AX done
-                    {fun (x: I + X) w' =>
-                       match x with
-                       | inl i' => Ri i' w' /\ Rv (i', w') (i, w)
-                       | inr r' => not_done w' /\ φ w' /\ Rr r' w'
-                       end})>) ->
-    well_founded Rv ->
-    Ri i w ->
-    <( {iter k i}, w |= base φ AU done Rr )>.
-  Proof.      
-    intros H WfR Hi.
-    generalize dependent k.
-    revert Hi.
+        <( {k i}, w |= φ AX ψ )> \/
+          <[ {k i}, w |= φ AX done
+                      {fun (lr: I + X) (w': World E) => exists i', lr = inl i' /\ Ri i' w' /\ Rv (i', w') (i, w)}]>) ->
+    <( {iter k i}, w |= φ AX ψ )>.
+  Proof with auto with ctl.
     remember (i, w) as P.
     replace i with (fst P) by now subst.
     replace w with (snd P) by now subst.
     clear HeqP i w.
+    intros WfR Hi H.
+    generalize dependent k.
     induction P using (well_founded_induction WfR);
       destruct P as (i, w); cbn in *. 
     rename H into HindWf.
     intros.
     unfold iter, MonadIter_ctree.
     rewrite unfold_iter.
-    eapply au_bind_r with
-      (R:=fun (x : I + X) (w' : World E) =>
-            match x with
-            | inl i' => Ri i' w' /\ Rv (i', w') (i, w)
-            | inr r' => not_done w' /\ φ w' /\ Rr r' w'
-            end); auto.
-    intros [i' | r] w'.            
-    - intros (Hi' & Hv). 
-      apply au_guard.
-      remember (i', w') as y.
-      replace i' with (fst y) by now subst.
-      replace w' with (snd y) by now subst.      
-      apply HindWf; inv Heqy; auto.
-    - intros [Hd (Hφ & HR)]; inv Hd.
-      + apply au_ret_l.
-        * rewrite ax_done; split; eauto with ctl.
-        * apply ctl_base; intuition. 
-      + apply au_ret_l.
-        * rewrite ax_done; split; eauto with ctl. 
-        * apply ctl_base; intuition. 
+    destruct (H _ _ Hi).
+    - now eapply ctll_bind_l.
+    - eapply axl_bind_r with
+        (R:=fun (lr: I + X) (w': World E) =>
+              exists i' : I, lr = inl i' /\ Ri i' w' /\ Rv (i', w') (i, w))... 
+      intros [i' | r] w'.            
+      + intros (j & Hinv & Hi' & Hv); inv Hinv.
+        rewrite sb_guard.
+        remember (j, w') as y.
+        replace j with (fst y) in Hi' |- * by now subst.
+        replace w' with (snd y) in Hi' |- * by now subst.
+        apply HindWf...
+      + intros (j & Hcontra & ?); inv Hcontra.
   Qed.
 
-  (*| Instead of a WF relation [Rv] a "ranking" function [f] |*)
-  Lemma au_iter_nat{X I} Ri Rr (f: I -> World E -> nat) (i: I) w (k: I -> ctree E (I + X)) φ:
-    (forall (i: I) w,
-        Ri i w ->
-        <( {k i}, w |= base φ AU AX done
-                    {fun (x: I + X) w' =>
-                       match x with
-                       | inl i' => Ri i' w' /\ f i' w' < f i w
-                       | inr r' => not_done w' /\ φ w' /\ Rr r' w'
-                       end})>) ->
-    Ri i w ->
-    <( {iter k i}, w |= base φ AU done Rr )>.
-  Proof.
-    intros.
-    eapply au_iter with Ri (ltof _ (fun '(i, w) => f i w));
-      auto.
-    apply well_founded_ltof.
-  Qed.
-
-  (* Well-founded induction on length of lists *)
-  Lemma au_iter_list{A X I} Ri Rr (f: I -> World E -> list A) (i: I) w (k: I -> ctree E (I + X)) φ:
-    (forall (i: I) w,
-        Ri i w ->
-        <( {k i}, w |= base φ AU AX done
-                    {fun (x: I + X) w' =>
-                       match x with
-                       | inl i' => Ri i' w' /\ length (f i' w') < length (f i w)
-                       | inr r' => not_done w' /\ φ w' /\ Rr r' w'
-                       end})>) ->
-    Ri i w ->
-    <( {iter k i}, w |= base φ AU done Rr )>.
-  Proof.
-    intros.
-    eapply au_iter_nat with
-      Ri (fun i w => length (f i w)); auto.
-  Qed.
-End CtlAuIter.
-
-(*| Combinators for [interp_state] |*)
-Section CtlAuState.
-  Context {E F S: Type} {HE: Encode E} {HF: Encode F}
-    (h: E ~> stateT S (ctree F)).
-
-  Theorem au_state_bind_l{X Y}: forall s w (t: ctree E Y) (k: Y -> ctree E X) φ,
-      <( {interp_state h t s}, w |= AF now φ )> ->
-      <( {interp_state h (x <- t ;; k x) s}, w |= AF now φ )>.
-  Proof.
-    intros.
-    rewrite interp_state_bind.
-    now apply au_bind_l.
-  Qed.  
-
-  Theorem au_state_bind_r{X Y}: forall s (t: ctree E Y) (k: Y -> ctree E X) w ψ φ (R: Y -> S -> World F -> Prop),
-      <( {interp_state h t s}, w |= base ψ AU AX done {fun '(y, s) => R y s} )> ->
-      (forall (y: Y) (s: S) w, R y s w ->
-          <( {interp_state h (k y) s}, w |= base ψ AU φ )>) ->
-      <( {interp_state h (x <- t ;; k x) s}, w |= base ψ AU φ )>.
-  Proof.
-    intros.
-    rewrite interp_state_bind.
-    apply au_bind_r with (R:=fun '(y, s) => R y s); auto.
-    intros [y s'] w' Hr; auto.
-  Qed.
-
-  Theorem au_state_bind_r_eq{X Y}: forall s s' (t: ctree E Y) (k: Y -> ctree E X) w w' ψ φ (r: Y),
-      <( {interp_state h t s}, w |= base ψ AU AX done={(r, s')} w' )> ->
-      <( {interp_state h (k r) s'}, w' |= base ψ AU φ )> ->
-      <( {interp_state h (x <- t ;; k x) s}, w |= base ψ AU φ )>.
-  Proof.
-    intros.
-    rewrite interp_state_bind.
-    apply au_bind_r_eq with (r, s') w'; auto. 
-  Qed.
-
-  Theorem au_state_iter{X I} s Ri (Rr: rel (X * S) (World F)) Rv (i: I) (k: I -> ctree E (I + X)) φ w:
-    (forall (i: I) w s,
-        Ri i w s ->
-        not_done w ->
-        <( {interp_state h (k i) s}, w |= base φ AU AX done
-          {fun '(x, s') w' => not_done w' /\
-             match x with
-             | inl i' => Ri i' w' s' /\ Rv (i', w', s') (i, w, s)
-             | inr r' => φ w' /\ Rr (r',s') w'
-             end})>) ->
+  Lemma axr_iter{X I} Ri (Rv: relation (I * World E)) (i: I) w (k: I -> ctree E (I + X)) (φ: ctll E) (ψ: ctlr E X):
     well_founded Rv ->
-    Ri i w s ->
-    not_done w ->
-    <( {interp_state h (Ctree.iter k i) s}, w |= base φ AU done Rr )>.
-  Proof.
-    intros H WfR Hi Hd.
+    Ri i w ->    
+    (forall (i: I) w,
+        Ri i w ->
+        <[ {k i}, w |= φ AX done
+                    {fun (lr: I + X) (w': World E) =>
+                       match lr with
+                       | inl i' => Ri i' w' /\ Rv (i', w') (i, w)
+                       | inr r => <[ {Ret r}, w' |= φ AX ψ ]>
+                       end} ]>) ->
+    <[ {iter k i}, w |= φ AX ψ ]>.
+  Proof with auto with ctl.
+    remember (i, w) as P.
+    replace i with (fst P) by now subst.
+    replace w with (snd P) by now subst.
+    clear HeqP i w.
+    intros WfR Hi H.
     generalize dependent k.
-    revert Hi.
-    remember (i, w, s) as P.
-    replace i with (fst (fst P)) by now subst.
-    replace w with (snd (fst P)) by now subst.
-    replace s with (snd P) by now subst.
-    replace w with (snd (fst P)) in Hd by now subst.
-    clear HeqP i w s.
     induction P using (well_founded_induction WfR);
-      destruct P as ((i, w), s); cbn in *. 
+      destruct P as (i, w); cbn in *. 
     rename H into HindWf.
     intros.
-    rewrite interp_state_unfold_iter.
-    eapply au_bind_r with (R:=fun '(r, s0) (w0 : World F) => not_done w0 /\
-                      match r with
-                      | inl i' => Ri i' w0 s0 /\ Rv (i', w0, s0) (i, w, s)
-                      | inr r' => φ w0 /\ Rr (r',s0) w0
-                      end); auto.
-    intros ([i' | r] & s') w'; cbn.
-    - intros (Hd' & Hi' & Hv).
-      apply au_guard.
-      remember (i', w',s') as y.
-      replace i' with (fst (fst y)) by now subst.
-      replace w' with (snd (fst y)) by now subst.
-      replace s' with (snd y) by now subst.      
-      apply HindWf; inv Heqy; auto.
-    - intros (Hd' & HR & Hr); inv Hd';
-        apply au_ret_l; auto with ctl;
-        rewrite ax_done; split; eauto with ctl.          
+    unfold iter, MonadIter_ctree.
+    rewrite unfold_iter.
+    destruct (H _ _ Hi).
+    - eapply axr_bind_r with
+        (R:=(fun (lr : I + X) (w' : World E) =>
+               match lr with
+               | inl i' => Ri i' w' /\ Rv (i', w') (i, w)
+               | inr r => <[ {Ret r}, w' |= φ AX ψ ]>
+               end))...
+      intros [i' | r] w'...
+      intros (Hi' & Hv). 
+      rewrite sb_guard.
+      remember (i', w') as y.
+      replace i' with (fst y) in Hi' |- * by now subst.
+      replace w' with (snd y) in Hi' |- * by now subst.
+      apply HindWf...
   Qed.
-    
-  (*| Instead of a WF relation [Rv] a "ranking" function [f] |*)
-  Lemma au_state_iter_nat{X I} (s: S) Ri (Rr: rel (X * S) (World F)) (f: I -> World F -> S -> nat) (i: I) φ w
-    (k: I -> ctree E (I + X)):
-    (forall (i: I) w s,
-        Ri i w s ->
-        not_done w ->
-        <( {interp_state h (k i) s}, w |= base φ AU AX done
-                                       {fun '(x, s') w' =>
-                                          not_done w' /\
-                                            match x with
-                                            | inl i' => Ri i' w' s' /\ f i' w' s' < f i w s
-                                            | inr r' => φ w' /\ Rr (r', s') w'
-                                            end})>) ->
-    Ri i w s ->
-    not_done w ->
-    <( {interp_state h (Ctree.iter k i) s}, w |= base φ AU done Rr )>.
-  Proof.
+
+  (* AU *)
+  Lemma aul_iter{X I} Ri (Rv: relation (I * World E)) (i: I) w (k: I -> ctree E (I + X)) (φ ψ: ctll E):
+    well_founded Rv ->
+    Ri i w ->    
+    (forall (i: I) w,
+        Ri i w ->
+        <( {k i}, w |= φ AU ψ )> \/
+          <[ {k i}, w |= φ AU AN done
+                      {fun (lr: I + X) (w': World E) => exists i', lr = inl i' /\ Ri i' w' /\ Rv (i', w') (i, w)}]>) ->
+    <( {iter k i}, w |= φ AU ψ )>.
+  Proof with auto with ctl.
+    remember (i, w) as P.
+    replace i with (fst P) by now subst.
+    replace w with (snd P) by now subst.
+    clear HeqP i w.
+    intros WfR Hi H.
+    generalize dependent k.
+    induction P using (well_founded_induction WfR);
+      destruct P as (i, w); cbn in *. 
+    rename H into HindWf.
     intros.
-    eapply au_state_iter with Ri (ltof _ (fun '(i, w, s) => f i w s)); auto.
-    apply well_founded_ltof.
+    unfold iter, MonadIter_ctree.
+    rewrite unfold_iter.
+    destruct (H _ _ Hi).
+    - now eapply ctll_bind_l.
+    - eapply aul_bind_r with
+        (R:=fun (lr: I + X) (w': World E) =>
+              exists i' : I, lr = inl i' /\ Ri i' w' /\ Rv (i', w') (i, w))... 
+      intros [i' | r] w'.            
+      + intros (j & Hinv & Hi' & Hv); inv Hinv.
+        rewrite sb_guard.
+        remember (j, w') as y.
+        replace j with (fst y) in Hi' |- * by now subst.
+        replace w' with (snd y) in Hi' |- * by now subst.
+        apply HindWf...
+      + intros (j & Hcontra & ?); inv Hcontra.
   Qed.
 
-End CtlAuState.
-
-(*| Combinators for [interp_state] with [writerE] |*)
-Section CtlAuStateList.
-  Context {E F A: Type} {HE: Encode E} {HF: Encode F} (h: E ~> stateT (list A) (ctree F)).
-
-  Lemma au_state_iter_list{X I} Ri (Rr: rel (X * list A) (World F)) (l: list A) w (i: I) (k: I -> ctree E (I + X)) φ :
-    (forall (i: I) w (l: list A),
-        Ri i w l ->
-        not_done w ->
-        <( {interp_state h (k i) l}, w |= base φ AU AX done
-                 {fun '(x, l') w' => not_done w' /\
-                    match x with
-                    | inl i' => Ri i' w' l' /\ length l' < length l
-                    | inr r' => φ w' /\ Rr (r', l') w'
-                    end})>) ->
-    Ri i w l ->
-    not_done w ->
-    <( {interp_state h (Ctree.iter k i) l}, w |= base φ AU done Rr )>.
-  Proof.
+  Lemma aur_iter{X I} Ri (Rv: relation (I * World E)) (i: I) w (k: I -> ctree E (I + X)) (φ: ctll E) (ψ: ctlr E X):
+    well_founded Rv ->
+    Ri i w ->    
+    (forall (i: I) w,
+        Ri i w ->
+        <[ {k i}, w |= φ AU AN done
+                    {fun (lr: I + X) (w': World E) =>
+                       match lr with
+                       | inl i' => Ri i' w' /\ Rv (i', w') (i, w)
+                       | inr r => <[ {Ret r}, w' |= ψ \/ φ AX ψ ]>
+                       end} ]>) ->
+    <[ {iter k i}, w |= φ AU ψ ]>.
+  Proof with auto with ctl.
+    remember (i, w) as P.
+    replace i with (fst P) by now subst.
+    replace w with (snd P) by now subst.
+    clear HeqP i w.
+    intros WfR Hi H.
+    generalize dependent k.
+    induction P using (well_founded_induction WfR);
+      destruct P as (i, w); cbn in *. 
+    rename H into HindWf.
     intros.
-    apply au_state_iter_nat with (Ri:=Ri) (f:=fun _ _ l => length l);
-      auto.
-  Qed.
-End CtlAuStateList.
-
-
-(*| Combinators for [interp_state] |*)
-Section CtlAgState.
-  Context {E F S: Type} {HE: Encode E} {HF: Encode F}
-    (h: E ~> stateT S (ctree F)).
-
-  Theorem ag_state_bind_l{X Y}: forall s w (t: ctree E Y) (k: Y -> ctree E X) φ,
-      <( {interp_state h t s}, w |= AG now φ )> ->
-      <( {interp_state h (x <- t ;; k x) s}, w |= AG now φ )>.
-  Proof.
-    intros.
-    rewrite interp_state_bind.
-    now apply ag_bind_l.
+    unfold iter, MonadIter_ctree.
+    rewrite unfold_iter.
+    eapply aur_bind_r with
+      (R:=(fun (lr : I + X) (w' : World E) =>
+             match lr with
+             | inl i' => Ri i' w' /\ Rv (i', w') (i, w)
+             | inr r => <[ {Ret r}, w' |= ψ \/ φ AX ψ ]>
+             end))...
+    intros [i' | r] w'...
+    intros (Hi' & Hv). 
+    rewrite sb_guard.
+    remember (i', w') as y.
+    replace i' with (fst y) in Hi' |- * by now subst.
+    replace w' with (snd y) in Hi' |- * by now subst.
+    apply HindWf...
+    apply aur_ret.
   Qed.
 
-  Theorem ag_state_bind_r{X Y}: forall s (t: ctree E Y) (k: Y -> ctree E X) w φ
-                                  (R: Y -> S -> World F -> Prop),
-      <( {interp_state h t s}, w |= now φ AU (AX done {fun '(x, s) w => R x s w}) )> ->
-      (forall (y: Y) (s: S) (w: World F),
-          R y s w ->
-          <( {interp_state h (k y) s}, w |= AG now φ )>) ->
-      <( {interp_state h (x <- t ;; k x) s} , w |= AG now φ )>.
-  Proof.
-    intros.
-    rewrite interp_state_bind.
-    apply ag_bind_r with (R:=fun '(x, s) w => R x s w); auto.
-    intros [y s'] w' Hr; auto.
-  Qed.
-
-  Theorem ag_state_iter{X I}: forall s (k: I -> ctree E (I + X)) w (x: I) φ R,
-      R x s ->        (* Iterator invariant: [x] in [R] *)
-      φ w ->          (* Worlds invariant: [φ w] *)
-      not_done w ->
-      (forall (x: I) (s: S) (w: World F),
-          R x s ->
-          φ w ->
-          not_done w ->
-          <( {interp_state h (k x) s}, w |= AX (now φ AU AX done
-             {fun (lr: (I+X) * S) (w: World F) =>
-                exists (i' : I) (s': S), lr = (inl i', s') /\ φ w /\
-                                      not_done w /\ R i' s'}))>) ->
-      <( {interp_state h (iter k x) s}, w |= AG now φ )>.
+  (* AG *)
+  Typeclasses Transparent sbisim.
+  Lemma ag_iter{X I} R (i: I) w (k: I -> ctree E (I + X)) (φ: ctll E) (ψ: ctlr E X):
+    R i w ->    
+    (forall (i: I) w,
+        R i w ->
+        <[ {k i}, w |= φ AX (φ AU AN done
+                    {fun (lr: I + X) (w': World E) =>
+                       exists (i': I), lr = inl i' /\ R i' w'}) ]>) ->
+    <( {iter k i}, w |= AG φ )>.
   Proof with auto with ctl.
     intros.
-    rewrite interp_state_unfold_iter.
-    generalize dependent x.
-    generalize dependent s.
-    generalize dependent w.
-    coinduction RR CIH; intros.
-    split; [apply ctl_now; now constructor|split].
-    - (* can_step *)
-      specialize (H2 _ _ _ H H0 H1).
-      cdestruct H2.
-      destruct Hs as (t' & w' & TR).
-      specialize (H2 _ _ TR).
-      apply can_step_bind_l with t' w'; auto.
-      cdestruct H2.
-      + now apply ax_done in H2 as (? & ?).
-      + now apply ctl_now in H2 as (? & ?). 
-    - intros t' w' TR.
-      apply ktrans_bind_inv in TR as
-          [(t0' & TR0 & Hd_ & Heq) | (x' & w0 & TRt0 & Hd & TRk)].
-      + (* [k x] steps *)
-        rewrite Heq; clear Heq t'.
-        apply (ft_t (ag_bind_now_ag φ
-                       (fun (lr: (I+X) * S) (w: World F) =>
-                          exists (i': I) (s': S), lr = (inl i', s') /\
-                                               φ w /\ not_done w /\ R i' s'))); cbn.
-        apply in_bind_ctx1.
-        * specialize (H2 _ _ _ H H0 H1) as HAX.
-          cdestruct HAX.
-          specialize (HAX _ _ TR0).
-          apply HAX.
-        * intros (lr' & s_) w_ (i & s' & Hinv & Hφ & Hd' & HR'); inv Hinv.
-          rewrite sb_guard.
-          setoid_rewrite interp_state_unfold_iter.
-          apply CIH...
-      + (* [k x] returns *)        
-        specialize (H2 _ _ _ H H0 H1) as HAX.        
-        cdestruct HAX.
-        specialize (HAX _ _ TRt0).
-        apply au_stuck in HAX.
-        cdestruct HAX.
-        now apply can_step_stuck in Hs0.
-  Qed.        
-End CtlAgState.
-
-Section CtlAgW.
-  Context {E Σ W: Type} {HE: Encode E} (h:E ~> stateT Σ (ctreeW W)). 
-
-  Theorem ag_iterW{X I}: forall (i: I) (σ: Σ) (w: W) (k: I -> ctree E (I + X)) φ R,
-      R i σ ->       (* Iterator & state invariant [R] *)
-      φ w ->         (* Goal Invariant [φ] *)
-      (forall (i: I) (σ: Σ) (w: W),
-          R i σ ->
-          φ w ->
-          <( {interp_state h (k i) σ}, {Obs (Log w) tt} |=
-              AX (visW φ AU AX
-                    (finishW {fun (lr: I + X) (σ: Σ) (w: W) =>
-                                exists (i: I), lr = inl i /\ R i σ /\ φ w})))>) ->
-      <( {interp_state h (iter k i) σ}, {Obs (Log w) tt} |= AG visW φ )>.
-  Proof with eauto with ctl.
-    setoid_rewrite ctl_vis_now.
-    setoid_rewrite ctl_finish_done.
-    intros.
-    rewrite interp_state_unfold_iter.
-    generalize dependent σ.
+    (* coinductive case *)
     generalize dependent i.
-    generalize dependent w.    
+    generalize dependent w.
+    unfold iter, MonadIter_ctree.
+    setoid_rewrite sb_unfold_iter.
     coinduction RR CIH; intros.
-    split; [apply ctl_now; eauto with ctl |split].
-    - (* can_step *)
-      specialize (H1 _ _ _ H H0).
-      cdestruct H1.
-      destruct Hs as (t' & w' & TR).
-      specialize (H1 _ _ TR).
-      apply can_step_bind_l with t' w'...
-      cdestruct H1.
-      + apply ax_done in H1 as (? & ?)...
-      + apply ctl_now in H1; destruct H1...
+    specialize (H0 _ _ H) as H0'.
+    cdestruct H0'.
+    split2.
+    - now apply ctll_bind_l.
+    - destruct Hs as (k' & wk & TRk).
+      apply can_step_bind_l with k' wk...
+      specialize (H0' _ _ TRk).
+      now apply aur_not_done in H0'.
     - intros t' w' TR.
       apply ktrans_bind_inv in TR as
           [(t0' & TR0 & Hd_ & Heq) | (x' & w0 & TRt0 & Hd & TRk)].
       + (* [k x] steps *)
         rewrite Heq; clear Heq t'.
-        apply (ft_t (ag_bind_now_ag
-                       (fun w => (exists (e : writerE W) (v : encode e),
-                                  w = Obs e v /\
-                                    (let 'Log v0 as x := e return (encode x -> Prop) in
-                                     fun 'tt => φ v0) v))
-                       (fun (x : (I + X) * Σ) (w : World (writerE W)) =>
-                        exists (e : writerE W) (v : encode e),
-                          w = Obs e v /\
-                          (let
-                           '(x0, s) := x in
-                            fun pat0 : writerE _ =>
-                            let
-                              'Log w0 as u := pat0 return (encode u -> Prop) in
-                            fun 'tt => exists i' : I, x0 = inl i' /\ R i' s /\ φ w0)
-                            e v))); cbn.
+        apply (ft_t (ag_bind_ag φ
+                       (fun (lr: I+X) (w0: World E) => exists i' : I, lr = inl i' /\ R i' w0))).
         apply in_bind_ctx1.
-        * specialize (H1 _ _ _ H H0) as HAX.
-          cdestruct HAX.
-          specialize (HAX _ _ TR0).
-          apply HAX.
-        * intros (lr' & s_) w_ ([σ'] & [] & ? & ? & i' & ? & ?); subst.
-          unfold Classes.iter, MonadIter_ctree.          
-          apply (ft_t (mequ_clos_cag (KS:=KripkeSetoidSBisim))); cbn.
-          econstructor.
-          rewrite sb_guard.
-          rewrite interp_state_unfold_iter.
-          reflexivity.
-          reflexivity.
+        * now apply H0'. 
+        * intros [l | r] w_ (? & Hinv & HR); inv Hinv.
+          rewrite sb_unfold_iter.
           apply CIH...
       + (* [k x] returns *)        
-        specialize (H1 _ _ _ H H0) as HAX.        
-        cdestruct HAX.
-        specialize (HAX _ _ TRt0).
-        apply au_stuck in HAX.
-        cdestruct HAX.
-        now apply can_step_stuck in Hs0.
-  Qed.        
+        specialize (H0' _ _ TRt0) as HAX.
+        now apply aur_stuck, axr_stuck in HAX.
+  Qed.
 
-End CtlAgW.
+  (* EG *)
+  Lemma eg_iter{X I} R (i: I) w (k: I -> ctree E (I + X)) (φ: ctll E) (ψ: ctlr E X):
+    R i w ->    
+    (forall (i: I) w,
+        R i w ->
+        <[ {k i}, w |= φ EX (φ EU EN done
+                    {fun (lr: I + X) (w': World E) =>
+                       exists (i': I), lr = inl i' /\ R i' w'}) ]>) ->
+    <( {iter k i}, w |= EG φ )>.
+  Proof with auto with ctl.
+    intros.
+    (* coinductive case *)
+    generalize dependent i.
+    generalize dependent w.
+    unfold iter, MonadIter_ctree.
+    setoid_rewrite sb_unfold_iter.
+    coinduction RR CIH; intros.
+    specialize (H0 _ _ H) as H0'.
+    cdestruct H0'.
+    split.
+    - now apply ctll_bind_l.
+    - exists (lr <- t;; match lr with
+                 | inl l => Ctree.iter k l
+                 | inr r => Ret r
+                  end), w0; split.
+      + apply ktrans_bind_r...
+        now apply eur_not_done in H0'.
+      + apply (ft_t (eg_bind_eg φ
+                       (fun (lr: I+X) (w0: World E) => exists i' : I, lr = inl i' /\ R i' w0))).
+        apply in_bind_ctx1.
+        * now apply H0'. 
+        * intros [l | r] w_ (? & Hinv & HR); inv Hinv.
+          rewrite sb_unfold_iter.
+          apply CIH...
+  Qed.
+End IterLemmas.
